Refactor DB code.

store/db.v
@@ -1,4 +1,4 @@
-From stdpp Require Import base countable gmap.
+From stdpp Require Import base gmap.
 From mathcomp Require Import ssreflect.
 From stdpp Require Import namespaces.
 From iris.algebra Require Import agree auth csum gset gmap excl frac.
@@ -6,7 +6,7 @@ From iris.algebra Require Import max_prefix_list.
 From iris.heap_lang Require Import notation proofmode.
 From iris.heap_lang.lib Require Import lock ticket_lock.
 From cryptis Require Import lib version term cryptis primitives tactics.
-From cryptis.store Require Import impl shared.
+From cryptis Require Import role session pk_auth pk_dh.
 
 Set Implicit Arguments.
 Unset Strict Implicit.
@@ -29,6 +29,50 @@ Class dbGS Σ := DbGS {
 
 Local Existing Instance db_inG.
 
+Module DB.
+
+Definition new : val := λ: <>,
+  let: "kvs" := ref [] in
+  let: "lock" := newlock #() in
+  ("kvs", "lock").
+
+Definition find : val := λ: "kvs" "k",
+  let: "res" := find_list (λ: "kv", eq_term (Fst "kv") "k") "kvs" in
+  match: "res" with
+    SOME "res" => SOME (Snd "res")
+  | NONE => NONE
+  end.
+
+Definition while_locked : val := λ: "db" "f",
+  let: "kvs" := Fst "db" in
+  let: "lock" := Snd "db" in
+  acquire "lock";;
+  let: "res" := "f" "kvs" in
+  release "lock";;
+  "res".
+
+Definition set : val := λ: "db" "k" "v",
+  while_locked "db" (λ: "kvs",
+      "kvs" <- ("k", "v") :: !"kvs";;
+      #()
+  ).
+
+Definition get : val := λ: "db" "k",
+  while_locked "db" (λ: "kvs",
+      match: find !"kvs" "k" with
+        SOME "res" => "res"
+      | NONE => #() (* Error *)
+      end
+  ).
+
+Definition create : val := λ: "db" "k" "v",
+  while_locked "db" (λ: "kvs",
+    match: find !"kvs" "k" with
+      SOME <> => #false
+    | NONE => "kvs" <- ("k", "v") :: !"kvs";; #true
+    end
+  ).
+
 Section Verif.
 
 Context `{!cryptisGS Σ, !heapGS Σ, !dbGS Σ}.
@@ -38,34 +82,31 @@ Implicit Types (γ : gname) (l : loc) (t : term) (v : val).
 Implicit Types (kvs : list (term * term)) (db : gmap term term).
 
 Definition is_alist kvs db : Prop :=
-  ∀ k, db !! k = snd <$> find (λ p, bool_decide (p.1 = k)) kvs.
+  ∀ k, db !! k = snd <$> List.find (λ p, bool_decide (p.1 = k)) kvs.
 
 Definition stores_db l db : iProp :=
   ∃ kvs, l ↦ repr kvs ∗ ⌜is_alist kvs db⌝.
 
-Definition db_auth db : dbUR :=
-  ● (Excl <$> db).
+Definition auth db : dbUR := ● (Excl <$> db).
+Definition frag db : dbUR := ◯ (Excl <$> db).
 
-Definition db_frag db : dbUR :=
-  ◯ (Excl <$> db).
-
-Lemma valid_db_auth db : ✓ db_auth db.
+Lemma valid_auth db : ✓ auth db.
 Proof.
 apply/auth_auth_valid => k; rewrite lookup_fmap; by case: (db !! k).
 Qed.
 
-Lemma valid_db_frag db : ✓ db_frag db.
+Lemma valid_frag db : ✓ frag db.
 Proof.
 apply/auth_frag_valid => k; rewrite lookup_fmap; by case: (db !! k).
 Qed.
 
-Hint Resolve valid_db_auth : core.
+Hint Resolve valid_auth : core.
 
-Lemma db_auth_db_frag_valid db1 db2 :
-  ✓ (db_auth db1 ⋅ db_frag db2) →
+Lemma auth_frag_valid db1 db2 :
+  ✓ (auth db1 ⋅ frag db2) →
   ∀ t1 t2, db2 !! t1 = Some t2 -> db1 !! t1 = Some t2.
 Proof.
-rewrite /db_auth /db_frag => /auth_both_valid_discrete [incl_12 valid_1] t1 t2.
+rewrite /auth /frag => /auth_both_valid_discrete [incl_12 valid_1] t1 t2.
 move: incl_12; rewrite lookup_included; move/(_ t1).
 rewrite !lookup_fmap => incl_12 db2_t1.
 rewrite db2_t1 /= in incl_12.
@@ -74,33 +115,33 @@ case db1_t1: (db1 !! t1) => [t2'|] /= in incl_12 *.
 - by case/option_included: incl_12 => // - [] ? [] ? [] ? [] ?.
 Qed.
 
-Lemma db_auth_db_frag1_valid db t1 t2 :
-  ✓ (db_auth db ⋅ db_frag {[t1 := t2]}) →
+Lemma auth_frag1_valid db t1 t2 :
+  ✓ (auth db ⋅ frag {[t1 := t2]}) →
   db !! t1 = Some t2.
 Proof.
-move=> valid_12; apply: (db_auth_db_frag_valid valid_12).
+move=> valid_12; apply: (auth_frag_valid valid_12).
 by rewrite lookup_singleton.
 Qed.
 
-Lemma db_auth_db_frag_update db t1 t2 t2' :
-  db_auth db ⋅ db_frag {[t1 := t2]} ~~>
-  db_auth (<[t1 := t2']> db) ⋅ db_frag {[t1 := t2']}.
+Lemma auth_frag_update db t1 t2 t2' :
+  auth db ⋅ frag {[t1 := t2]} ~~>
+  auth (<[t1 := t2']> db) ⋅ frag {[t1 := t2']}.
 Proof.
 apply/auth_update; rewrite fmap_insert !map_fmap_singleton.
 apply: singleton_local_update_any => x _.
 by apply: exclusive_local_update.
 Qed.
 
-Lemma db_auth_db_frag_alloc db t1 t2 :
+Lemma auth_frag_alloc db t1 t2 :
   db !! t1 = None ->
-  db_auth db ~~> db_auth (<[t1 := t2]> db) ⋅ db_frag {[t1 := t2]}.
+  auth db ~~> auth (<[t1 := t2]> db) ⋅ frag {[t1 := t2]}.
 Proof.
 move=> db_t1. apply/auth_update_alloc; rewrite fmap_insert map_fmap_singleton.
 by apply: alloc_singleton_local_update => //; rewrite lookup_fmap db_t1.
 Qed.
 
 Definition db_res γ l : iProp :=
-  ∃ db, stores_db l db ∗ own γ (db_auth db).
+  ∃ db, stores_db l db ∗ own γ (auth db).
 
 Definition is_db v : iProp :=
   ∃ l vlock γkvs γlock,
@@ -122,7 +163,7 @@ wp_bind (ref _)%E; iApply wp_alloc => //.
 iIntros "!> %l [Hl meta]".
 rewrite (meta_token_difference _ (↑(nroot.@"kvs")) _) //.
 iDestruct "meta" as "[meta_kvs meta]".
-iMod (own_alloc (db_auth ∅)) as "[%γkvs own_γkvs]" => //.
+iMod (own_alloc (auth ∅)) as "[%γkvs own_γkvs]" => //.
 iMod (meta_set _ _ γkvs (nroot.@"kvs") with "meta_kvs") as "#meta_kvs" => //.
 wp_pures; wp_bind (newlock _).
 iApply (newlock_spec (db_res γkvs l) with "[Hl own_γkvs]").
@@ -147,17 +188,17 @@ iApply (wp_find_list (λ x, bool_decide (x.1 = t)) _ kvs) => //.
 { move=> [k t']; iIntros "%Φ' _ Hpost".
   wp_pures. iApply wp_eq_term. by iApply "Hpost". }
 iIntros "!> _"; rewrite kvs_db.
-by case: find => [[k' t']|] /=; wp_pures; iApply "Hpost".
+by case: List.find => [[k' t']|] /=; wp_pures; iApply "Hpost".
 Qed.
 
-Lemma wp_with_locked_db v Φ (f : val) :
+Lemma wp_while_locked v Φ (f : val) :
   (∀ γkvs l vlock,
       ⌜v = (#l, vlock)%V⌝ -∗
       meta l (nroot.@"kvs") γkvs -∗
       db_res γkvs l -∗
       WP f #l {{ res, Φ res ∗ db_res γkvs l }}) -∗
   is_db v -∗
-  WP DB.with_locked_db v f {{ res, Φ res }}.
+  WP while_locked v f {{ res, Φ res }}.
 Proof.
 iIntros "wp_f (%l & %vlock & %γkvs & %γloc & -> & #m_kvs & #m_lock & #lock)".
 wp_lam; wp_pures.
@@ -172,16 +213,16 @@ wp_pures; wp_bind (release _); iApply (release_spec with "[locked db_res]").
 iIntros "!> _"; wp_pures; eauto.
 Qed.
 
-Definition db_mapsto v t1 t2 : iProp :=
+Definition mapsto v t1 t2 : iProp :=
   ∃ l vlock γkvs,
     ⌜v = (#l, vlock)%V⌝ ∗
     meta l (nroot.@"kvs") γkvs ∗
-    own γkvs (db_frag {[t1 := t2]}).
+    own γkvs (frag {[t1 := t2]}).
 
-Lemma db_mapsto_inv l v γkvs t1 t2 :
-  db_mapsto (#l, v)%V t1 t2 -∗
+Lemma mapsto_inv l v γkvs t1 t2 :
+  mapsto (#l, v)%V t1 t2 -∗
   meta l (nroot.@"kvs") γkvs -∗
-  own γkvs (db_frag {[t1 := t2]}).
+  own γkvs (frag {[t1 := t2]}).
 Proof.
 iIntros "(%l' & %v' & %γkvs' & %E & #meta' & own) #meta".
 case: E => <- _ {l' v'}.
@@ -198,24 +239,24 @@ move=> kvs_db k' /=; case: bool_decide_reflect => [<-|ne].
 Qed.
 
 Lemma wp_set v t1 t2 t2' :
-  {{{ is_db v ∗ db_mapsto v t1 t2 }}}
+  {{{ is_db v ∗ mapsto v t1 t2 }}}
     DB.set v t1 t2'
-  {{{ RET #(); db_mapsto v t1 t2' }}}.
+  {{{ RET #(); mapsto v t1 t2' }}}.
 Proof.
 iIntros "%Φ [#vP t1_t2] Hpost".
-wp_lam; wp_pures; iApply (wp_with_locked_db with "[t1_t2 Hpost] vP").
+wp_lam; wp_pures; iApply (wp_while_locked with "[t1_t2 Hpost] vP").
 iIntros "%γkvs %l %vlock -> #m_kvs lP".
-iPoseProof (db_mapsto_inv with "t1_t2 m_kvs") as "t1_t2".
+iPoseProof (mapsto_inv with "t1_t2 m_kvs") as "t1_t2".
 iDestruct "lP" as "(%db & (%kvs & l_kvs & %kvs_db) & dbP)".
 iPoseProof (own_valid_2 with "dbP t1_t2") as "%valid_12".
-have {valid_12} db_t1 := db_auth_db_frag1_valid valid_12.
+have {valid_12} db_t1 := auth_frag1_valid valid_12.
 wp_pures. wp_load. wp_pures. change (t1, t2')%V with (repr (t1, t2')).
 (* FIXME: The wp_cons tactic cannot proceed here because it undoes the previous
    change, which brings the goal to a shape where the tac_wp_cons lemma does not
    apply. *)
 wp_bind (_ :: _)%E. iApply (wp_cons _ (t1, t2') kvs). wp_store.
 iMod (own_update_2 with "dbP t1_t2") as "Hown".
-  exact: (db_auth_db_frag_update t2').
+  exact: (auth_frag_update t2').
 iDestruct "Hown" as "[dbP t1_t2]".
 iModIntro. iSplitL "Hpost t1_t2".
 - iApply "Hpost". iExists l, vlock, γkvs; eauto.
@@ -224,17 +265,17 @@ iModIntro. iSplitL "Hpost t1_t2".
 Qed.
 
 Lemma wp_get v t1 t2 :
-  {{{ is_db v ∗ db_mapsto v t1 t2 }}}
+  {{{ is_db v ∗ mapsto v t1 t2 }}}
     DB.get v t1
-  {{{ RET (repr t2); db_mapsto v t1 t2 }}}.
+  {{{ RET (repr t2); mapsto v t1 t2 }}}.
 Proof.
 iIntros "%Φ [#vP t1_t2] Hpost".
-wp_lam; wp_pures; iApply (wp_with_locked_db with "[t1_t2 Hpost] vP").
+wp_lam; wp_pures; iApply (wp_while_locked with "[t1_t2 Hpost] vP").
 iIntros "%γkvs %l %vlock -> #m_kvs lP".
-iPoseProof (db_mapsto_inv with "t1_t2 m_kvs") as "t1_t2".
+iPoseProof (mapsto_inv with "t1_t2 m_kvs") as "t1_t2".
 iDestruct "lP" as "(%db & (%kvs & l_kvs & %kvs_db) & dbP)".
 iPoseProof (own_valid_2 with "dbP t1_t2") as "%valid_12".
-have {valid_12} db_t1 := db_auth_db_frag1_valid valid_12.
+have {valid_12} db_t1 := auth_frag1_valid valid_12.
 wp_pures. wp_load. wp_bind (DB.find _ _)%E. iApply wp_find; eauto.
 iIntros "!> _". rewrite db_t1. wp_pures. iModIntro.
 iSplitL "Hpost t1_t2".
@@ -246,10 +287,10 @@ Lemma wp_create v t1 t2 :
   {{{ is_db v }}}
     DB.create v t1 t2
   {{{ (b : bool), RET #b;
-      if b then db_mapsto v t1 t2 else True }}}.
+      if b then mapsto v t1 t2 else True }}}.
 Proof.
 iIntros "%Φ #vP Hpost".
-wp_lam; wp_pures. iApply (wp_with_locked_db with "[Hpost] vP").
+wp_lam; wp_pures. iApply (wp_while_locked with "[Hpost] vP").
 iIntros "%γkvs %l %vlock -> #m_kvs lP".
 iDestruct "lP" as "(%db & (%kvs & l_kvs & %kvs_db) & dbP)".
 wp_pures. wp_load. wp_bind (DB.find _ _)%E. iApply wp_find; eauto.
@@ -259,7 +300,7 @@ iIntros "!> _". case db_t1: (db !! t1) => [t2'|]; wp_pures.
 wp_load. wp_pures. change (t1, t2)%V with (repr (t1, t2)).
 wp_bind (_ :: _)%E. iApply (wp_cons _ _ kvs). wp_store.
 iMod (own_update with "dbP") as "Hown".
-{ exact: (db_auth_db_frag_alloc t2). }
+{ exact: (auth_frag_alloc t2). }
 iDestruct "Hown" as "[dbP t1_t2]".
 iModIntro. iSplitL "Hpost t1_t2".
 - iApply "Hpost". iExists l, vlock, γkvs; iFrame. by eauto.
@@ -267,3 +308,5 @@ iModIntro. iSplitL "Hpost t1_t2".
 Qed.
 
 End Verif.
+
+End DB.
